\documentclass{article}
\title{Line Amid Two Points}
\begin{document}
\newcommand{\en}{\phantom{N}}
\maketitle
\section{Definition of ``Amid''}
The follwing defines ``amid'' with respect to a line and two points.
In particular, the existence of a centroid of the two points plays no role.
$$l\equiv \mathrm{line}(c\ a\ b), 0<a^2+b^2$$
\en\\
$$v\equiv \mathrm{vec\ list}\ l$$
\en\\
$$p_1\equiv \mathrm{point}(x_1\en y_1)$$
$$p_2\equiv \mathrm{point}(x_2\en y_2)$$
\en\\
$$u_1\equiv \mathrm{vec}(1\en x_1\en y_1)$$
$$u_2\equiv \mathrm{vec}(1\en x_2\en y_2)$$
\en\\
$$k_1\equiv v\cdot u_1$$
$$k_2\equiv v\cdot u_2$$
\en\\
line $l$ is ``amid'' points $p_1$ and $p_2\Leftrightarrow k_1=-k_2$.
\newpage
\section{Line Amid Two Points}
The line $l, \mathrm{line}(-ax_1-ax_2-by_1-by_2\en 2a\en2b), 0<a^2+b^2$ is amid
$\mathrm{point}(x_1\en y_1)$ and
$\mathrm{point}(x_2\en y_2)$.

\paragraph{Proof.}
Let $k_1=$
$$\mathrm{vec}(-ax_1-ax_2-by_1-by_2\en 2a\en2b)\cdot \mathrm{vec}(1\en x_1\en y_1)$$
$$=$$
$$-ax_1-ax_2-by_1-by_2+2ax_1+2by_1$$
$$=$$
$$ax_1-ax_2+by_1-by_2$$
And let $k_2=$
$$\mathrm{vec}(-ax_1-ax_2-by_1-by_2\en 2a\en2b)\cdot \mathrm{vec}(1\en x_2\en y_2)$$
$$=$$
$$-ax_1-ax_2-by_1-by_2+2ax_2+2by_2$$
$$=$$
$$-ax_1+ax_2-by_1+by_2$$
$k_1=-k_2$. \textsc{qed}
\end{document}
